spark2cmproofs.v
@@ -8,6 +8,8 @@ Require Ctypes.
 Require Import symboltable.
 Require Import semantics.
 Require Import semantics_properties.
+Require Import Sorted.
+Require Import Relations.
 
 Lemma wordsize_ok : wordsize = Integers.Int.wordsize.
 Proof.
@@ -38,6 +40,25 @@ Lemma min_signed_ok: min_signed = Integers.Int.min_signed.
 Proof.
   reflexivity.
 Qed.
+
+(* All element of a sorted list are smaller or equal to the first
+   element. If the ordering is reflexive. *)
+Lemma increasing_order_In A :
+  forall (ord:A -> A -> Prop) (stk:list A) (hd:A),
+    StronglySorted ord (hd::stk) ->
+    Forall (fun elt => elt = hd \/ ord hd elt) (hd::stk).
+Proof.
+  !intros.
+  !inversion H.
+  constructor 2.
+  - left;reflexivity.
+  - apply Forall_forall.
+    !intros.
+    right.
+    rewrite Forall_forall in H3.
+    auto.
+Qed.
+
 
 Import Symbol_Table_Module.
 Open Scope error_monad_scope.
@@ -108,6 +129,10 @@ Definition type_of_name (stbl:symboltable) (nme:name): res type :=
 (** Hypothesis renaming stuff *)
 Ltac rename_hyp1 h th :=
   match th with
+    | ?min <= ?x and ?x < ?max => fresh "h_" x "_bounded_" min "_" max 
+    | ?min <= ?x and ?x < ?max => fresh "h_" x "_bounded_"
+    | ?min <= ?x and ?x < ?max => fresh "h_bounded"
+
     | fetch_var_type _ _ = Error _ => fresh "heq_fetch_var_type_ERR"
     | fetch_var_type _ _ = _ => fresh "heq_fetch_var_type"
     | fetch_exp_type _ _ = Error _ => fresh "heq_fetch_exp_type_ERR"
@@ -164,6 +189,30 @@ Ltac rename_hyp1 h th :=
     | in_bound _ _ _ => fresh "h_inbound"
     | do_division_check _ _ (Run_Time_Error _) => fresh "h_do_division_check_RTE"
     | do_division_check _ _ _ => fresh "h_do_division_check"
+
+    | CompilEnv.fetchG ?id ?CE = _ => fresh "heq_CEfetchG_" id "_" CE
+    | CompilEnv.fetchG ?id _ = _ => fresh "heq_CEfetchG_" id
+    | CompilEnv.fetchG _ _ = Some _ => fresh "heq_CEfetchG"
+    | CompilEnv.fetchG _ _ = None => fresh "heq_CMfetchG_none"
+
+    | CompilEnv.fetch ?id ?CE = _ => fresh "heq_CEfetch_" id "_" CE
+    | CompilEnv.fetch ?id _ = _ => fresh "heq_CEfetch_" id
+    | CompilEnv.fetch _ _ = Some _ => fresh "heq_CEfetch"
+    | CompilEnv.fetch _ _ = None => fresh "heq_CMfetch_none"
+
+    | CompilEnv.frameG ?id ?CE = _ => fresh "heq_CEframeG_" id "_" CE
+    | CompilEnv.frameG ?id _ = _ => fresh "heq_CEframeG_" id
+    | CompilEnv.frameG _ _ = Some _ => fresh "heq_CEframeG"
+    | CompilEnv.frameG _ _ = None => fresh "heq_CMframeG_none"
+
+    | CompilEnv.level_of_top ?ce = None => fresh "heq_lvloftop_none_" ce
+    | CompilEnv.level_of_top ?ce = None => fresh "heq_lvloftop_none"
+    | CompilEnv.level_of_top ?ce = Some ?s => fresh "heq_lvloftop_" ce "_" s
+    | CompilEnv.level_of_top ?ce = ?s => fresh "heq_lvloftop_" ce "_" s
+    | CompilEnv.level_of_top ?ce = _ => fresh "heq_lvloftop_" ce
+    | CompilEnv.level_of_top _ = Some ?s => fresh "heq_lvloftop_" s
+    | CompilEnv.level_of_top _ = _ => fresh "heq_lvloftop"
+                                       
     (* TODO: remove when we remove type_of_name by the real one. *)
     | type_of_name _ _ = Error _ => fresh "heq_type_of_name_ERR"
     | type_of_name _ _ = _ => fresh "heq_type_of_name"
@@ -175,9 +224,7 @@ Lemma transl_literal_ok :
   forall g (l:literal) v,
     eval_literal l (Normal v) ->
     forall sp,
-    exists v',
-      transl_value v = OK v'
-      /\ eval_constant g sp (transl_literal l) = Some v'.
+      eval_constant g sp (transl_literal l) = Some (transl_value v).
 Proof.
   !intros.
   !destruct l;simpl in *.
@@ -224,6 +271,12 @@ Ltac inv_rtc :=
   repeat
     progress
     (try match goal with
+           | H: do_run_time_check_on_binop ?op Undefined _ (Normal _) |- _ => now inversion H
+           | H: do_run_time_check_on_binop ?op _ Undefined (Normal _) |- _ => now inversion H
+           | H: do_run_time_check_on_binop ?op _ (ArrayV _) (Normal _) |- _ => now inv_if_intop op H
+           | H: do_run_time_check_on_binop ?op (ArrayV _) _ (Normal _) |- _ => now inv_if_intop op H
+           | H: do_run_time_check_on_binop ?op _ (RecordV _) (Normal _) |- _ => now inv_if_intop op H
+           | H: do_run_time_check_on_binop ?op (RecordV _) _ (Normal _) |- _ => now inv_if_intop op H
            | H: do_run_time_check_on_binop ?op _ (Bool _) (Normal _) |- _ => inv_if_intop op H
            | H: Math.binary_operation ?op _ (Bool _) = (Some _) |- _ => inv_if_intop op H
            | H: do_run_time_check_on_binop ?op (Bool _) _ (Normal _) |- _ => inv_if_intop op H
@@ -252,9 +305,9 @@ Ltac inv_rtc :=
     when they don't raise a runtime error, like Compcert ones. *)
 
 Lemma not_ok: forall v1 v0 x,
-                     transl_value v1 = OK x ->
+                     transl_value v1 = x ->
                      Math.unary_not v1 = Some v0 ->
-                     transl_value v0 = OK (Values.Val.notbool x).
+                     transl_value v0 = (Values.Val.notbool x).
 Proof.
   !intros.
   !destruct v1;try discriminate;simpl in *.
@@ -275,10 +328,10 @@ Qed.
 
 
 Lemma and_ok: forall v1 v2 v0 x x0,
-                     transl_value v1 = OK x ->
-                     transl_value v2 = OK x0 ->
+                     transl_value v1 = x ->
+                     transl_value v2 = x0 ->
                      Math.and v1 v2 = Some v0 ->
-                     transl_value v0 = OK (Values.Val.and x x0).
+                     transl_value v0 = (Values.Val.and x x0).
 Proof.
   !intros.
   !destruct v1;try discriminate; !destruct v2;try discriminate;simpl in *.
@@ -290,10 +343,10 @@ Proof.
 Qed.
 
 Lemma or_ok: forall v1 v2 v0 x x0,
-                     transl_value v1 = OK x ->
-                     transl_value v2 = OK x0 ->
+                     transl_value v1 = x ->
+                     transl_value v2 = x0 ->
                      Math.or v1 v2 = Some v0 ->
-                     transl_value v0 = OK (Values.Val.or x x0).
+                     transl_value v0 = (Values.Val.or x x0).
 Proof.
   !intros.
   !destruct v1;try discriminate; !destruct v2;try discriminate;simpl in *.
@@ -326,10 +379,10 @@ Ltac rename_hyp ::= rename_hyp2.
 Lemma eq_ok: forall v1 v2 v0 x x0,
                check_overflow_value v1 -> 
                check_overflow_value v2 -> 
-               transl_value v1 = OK x ->
-               transl_value v2 = OK x0 ->
+               transl_value v1 = x ->
+               transl_value v2 = x0 ->
                Math.eq v1 v2 = Some v0 ->
-               transl_value v0 = OK (Values.Val.cmp Integers.Ceq x x0).
+               transl_value v0 = (Values.Val.cmp Integers.Ceq x x0).
 Proof.
   !intros.
   !destruct v1;try discriminate; !destruct v2;try discriminate;simpl in *.
@@ -344,6 +397,7 @@ Proof.
     reflexivity.
   - rewrite Fcore_Zaux.Zeq_bool_false;auto.
     unfold Values.Val.cmp.
+    subst.
     simpl.
     rewrite Integers.Int.eq_false.
     + reflexivity.
@@ -357,10 +411,10 @@ Qed.
 Lemma neq_ok: forall v1 v2 v0 x x0,
                check_overflow_value v1 -> 
                check_overflow_value v2 -> 
-               transl_value v1 = OK x ->
-               transl_value v2 = OK x0 ->
+               transl_value v1 = x ->
+               transl_value v2 = x0 ->
                Math.ne v1 v2 = Some v0 ->
-               transl_value v0 = OK (Values.Val.cmp Integers.Cne x x0).
+               transl_value v0 = (Values.Val.cmp Integers.Cne x x0).
 Proof.
   !intros.
   !destruct v1;try discriminate; !destruct v2;try discriminate;simpl in *.
@@ -375,6 +429,7 @@ Proof.
     reflexivity.
   - rewrite Zneq_bool_true;auto.
     unfold Values.Val.cmp.
+    subst.
     simpl.
     rewrite Integers.Int.eq_false.
     + reflexivity.
@@ -387,10 +442,10 @@ Qed.
 Lemma le_ok: forall v1 v2 v0 x x0,
                check_overflow_value v1 -> 
                check_overflow_value v2 -> 
-               transl_value v1 = OK x ->
-               transl_value v2 = OK x0 ->
+               transl_value v1 = x ->
+               transl_value v2 = x0 ->
                Math.le v1 v2 = Some v0 ->
-               transl_value v0 = OK (Values.Val.cmp Integers.Cle x x0).
+               transl_value v0 = (Values.Val.cmp Integers.Cle x x0).
 Proof.
   !intros.
   !destruct v1;try discriminate; !destruct v2;try discriminate;simpl in *.
@@ -399,6 +454,7 @@ Proof.
   !destruct (Z.le_decidable n n0).
   - rewrite Fcore_Zaux.Zle_bool_true;auto.
     unfold Values.Val.cmp.
+    subst.
     simpl.
     unfold Integers.Int.lt.
     rewrite Coqlib.zlt_false.
@@ -408,6 +464,7 @@ Proof.
       auto with zarith.
   - { rewrite Fcore_Zaux.Zle_bool_false.
       - unfold Values.Val.cmp.
+        subst.
         simpl.
         unfold Integers.Int.lt.
         rewrite Coqlib.zlt_true.
@@ -423,10 +480,10 @@ Qed.
 Lemma ge_ok: forall v1 v2 v0 x x0,
                check_overflow_value v1 -> 
                check_overflow_value v2 -> 
-               transl_value v1 = OK x ->
-               transl_value v2 = OK x0 ->
+               transl_value v1 = x ->
+               transl_value v2 = x0 ->
                Math.ge v1 v2 = Some v0 ->
-               transl_value v0 = OK (Values.Val.cmp Integers.Cge x x0).
+               transl_value v0 = (Values.Val.cmp Integers.Cge x x0).
 Proof.
   !intros.
   !destruct v1;try discriminate; !destruct v2;try discriminate;simpl in *.
@@ -436,6 +493,7 @@ Proof.
   !destruct (Z.le_decidable n0 n).
   - rewrite Fcore_Zaux.Zle_bool_true;auto.
     unfold Values.Val.cmp.
+    subst.
     simpl.
     unfold Integers.Int.lt.
     rewrite Coqlib.zlt_false.
@@ -445,6 +503,7 @@ Proof.
       auto with zarith.
   - { rewrite Fcore_Zaux.Zle_bool_false.
       - unfold Values.Val.cmp.
+        subst.
         simpl.
         unfold Integers.Int.lt.
         rewrite Coqlib.zlt_true.
@@ -459,10 +518,10 @@ Qed.
 Lemma lt_ok: forall v1 v2 v0 x x0,
                check_overflow_value v1 -> 
                check_overflow_value v2 -> 
-               transl_value v1 = OK x ->
-               transl_value v2 = OK x0 ->
+               transl_value v1 = x ->
+               transl_value v2 = x0 ->
                Math.lt v1 v2 = Some v0 ->
-               transl_value v0 = OK (Values.Val.cmp Integers.Clt x x0).
+               transl_value v0 = (Values.Val.cmp Integers.Clt x x0).
 Proof.
   !intros.
   !destruct v1;try discriminate; !destruct v2;try discriminate;simpl in *.
@@ -472,6 +531,7 @@ Proof.
   !destruct (Z.lt_decidable n n0).
   - rewrite Fcore_Zaux.Zlt_bool_true;auto.
     unfold Values.Val.cmp.
+    subst.
     simpl.
     unfold Integers.Int.lt.
     rewrite Coqlib.zlt_true.
@@ -480,6 +540,7 @@ Proof.
       rewrite Integers.Int.signed_repr;inv_rtc.
   - { rewrite Fcore_Zaux.Zlt_bool_false.
       - unfold Values.Val.cmp.
+        subst.
         simpl.
         unfold Integers.Int.lt.
         rewrite Coqlib.zlt_false.
@@ -493,10 +554,10 @@ Qed.
 Lemma gt_ok: forall v1 v2 v0 x x0,
                check_overflow_value v1 -> 
                check_overflow_value v2 -> 
-               transl_value v1 = OK x ->
-               transl_value v2 = OK x0 ->
+               transl_value v1 = x ->
+               transl_value v2 = x0 ->
                Math.gt v1 v2 = Some v0 ->
-               transl_value v0 = OK (Values.Val.cmp Integers.Cgt x x0).
+               transl_value v0 = (Values.Val.cmp Integers.Cgt x x0).
 Proof.
   !intros.
   !destruct v1;try discriminate; !destruct v2;try discriminate;simpl in *.
@@ -506,6 +567,7 @@ Proof.
   !destruct (Z.lt_decidable n0 n).
   - rewrite Fcore_Zaux.Zlt_bool_true;auto.
     unfold Values.Val.cmp.
+    subst.
     simpl.
     unfold Integers.Int.lt.
     rewrite Coqlib.zlt_true.
@@ -514,6 +576,7 @@ Proof.
       rewrite Integers.Int.signed_repr;inv_rtc.
   - { rewrite Fcore_Zaux.Zlt_bool_false.
       - unfold Values.Val.cmp.
+        subst.
         simpl.
         unfold Integers.Int.lt.
         rewrite Coqlib.zlt_false.
@@ -527,14 +590,15 @@ Qed.
 (* strangely this one does not need overflow preconditions *)
 Lemma unaryneg_ok :
   forall n v1 v,
-    transl_value v1 = OK n ->
+    transl_value v1 = n ->
     Math.unary_operation Unary_Minus v1 = Some v ->
-    transl_value v = OK (Values.Val.negint n).
+    transl_value v = (Values.Val.negint n).
 Proof.
   !intros.
   simpl in *.
   destruct v1;simpl in *;try discriminate.
   eq_same_clear.
+  subst.   
   simpl.
   rewrite Integers.Int.neg_repr.
   reflexivity.
@@ -569,14 +633,14 @@ Lemma add_ok :
     check_overflow_value v1 -> 
     check_overflow_value v2 -> 
     do_run_time_check_on_binop Plus v1 v2 (Normal v) ->
-    transl_value v1 = OK n1 ->
-    transl_value v2 = OK n2 ->
-    transl_value v = OK (Values.Val.add n1 n2).
+    transl_value v1 = n1 ->
+    transl_value v2 = n2 ->
+    transl_value v = (Values.Val.add n1 n2).
 Proof.
   !intros.
   simpl in *.
-  !destruct v1;simpl in *;try discriminate;eq_same_clear; try now inv_rtc.
-  !destruct v2;simpl in *; try discriminate;eq_same_clear; try now inv_rtc.
+  !destruct v1;simpl in *;try discriminate;eq_same_clear;subst;try now inv_rtc.
+  !destruct v2;simpl in *; try discriminate;eq_same_clear;subst; try now inv_rtc.
   - !invclear h_do_rtc_binop;simpl in *; eq_same_clear. 
     !invclear h_overf_check.
     int_simpl;auto;inv_rtc;auto 2.
@@ -587,14 +651,14 @@ Lemma sub_ok :
     check_overflow_value v1 -> 
     check_overflow_value v2 -> 
     do_run_time_check_on_binop Minus v1 v2 (Normal v) ->
-    transl_value v1 = OK n1 ->
-    transl_value v2 = OK n2 ->
-    transl_value v = OK (Values.Val.sub n1 n2).
+    transl_value v1 = n1 ->
+    transl_value v2 = n2 ->
+    transl_value v = (Values.Val.sub n1 n2).
 Proof.
   !intros.
   simpl in *.
-  !destruct v1;simpl in *;try discriminate;eq_same_clear; try now inv_rtc.
-  !destruct v2;simpl in *; try discriminate;eq_same_clear; try now inv_rtc.
+  !destruct v1;simpl in *;try discriminate;eq_same_clear;subst; try now inv_rtc.
+  !destruct v2;simpl in *; try discriminate;eq_same_clear;subst; try now inv_rtc.
   - !invclear h_do_rtc_binop;simpl in *; eq_same_clear. 
     !invclear h_overf_check.
     int_simpl;auto;inv_rtc;auto 2.
@@ -605,14 +669,14 @@ Lemma mult_ok :
     check_overflow_value v1 -> 
     check_overflow_value v2 -> 
     do_run_time_check_on_binop Multiply v1 v2 (Normal v) ->
-    transl_value v1 = OK n1 ->
-    transl_value v2 = OK n2 ->
-    transl_value v = OK (Values.Val.mul n1 n2).
+    transl_value v1 = n1 ->
+    transl_value v2 = n2 ->
+    transl_value v = (Values.Val.mul n1 n2).
 Proof.
   !intros.
   simpl in *.
-  !destruct v1;simpl in *;try discriminate;eq_same_clear; try now inv_rtc.
-  !destruct v2;simpl in *; try discriminate;eq_same_clear; try now inv_rtc.
+  !destruct v1;simpl in *;try discriminate;eq_same_clear;subst; try now inv_rtc.
+  !destruct v2;simpl in *; try discriminate;eq_same_clear;subst; try now inv_rtc.
   - !invclear h_do_rtc_binop;simpl in *; eq_same_clear. 
     !invclear h_overf_check.
     int_simpl;auto;inv_rtc;auto 2.
@@ -628,17 +692,17 @@ Lemma div_ok :
     check_overflow_value v1 -> 
     check_overflow_value v2 -> 
     do_run_time_check_on_binop Divide v1 v2 (Normal v) ->
-    transl_value v1 = OK n1 ->
-    transl_value v2 = OK n2 ->
-    transl_value v = OK n ->
+    transl_value v1 = n1 ->
+    transl_value v2 = n2 ->
+    transl_value v = n ->
     Values.Val.divs n1 n2 = Some n.
 Proof.
   !intros.
   simpl in *.
-  !destruct v1;simpl in *;try discriminate;try now inv_rtc.
-  !destruct v2;simpl in *; try discriminate;try now inv_rtc.
+  !destruct v1;subst;simpl in *;try discriminate;try now inv_rtc.
+  !destruct v2;subst;simpl in *; try discriminate;try now inv_rtc.
   rename n0 into v1.
-  rename n3 into v2.
+  rename n into v2.
   eq_same_clear;simpl in *.
   !invclear h_do_rtc_binop;simpl in *; eq_same_clear.
   { decompose [or] H;discriminate. }
@@ -683,7 +747,6 @@ Proof.
       !invclear heq;subst.
       inversion h_overf_check;subst.
       simpl in *.
-      inversion heq_transl_value.
       reflexivity.
   - unfold Integers.Int.zero.
     intro abs.
@@ -702,25 +765,25 @@ Lemma binary_operator_ok:
     check_overflow_value v1 ->
     check_overflow_value v2 ->
     do_run_time_check_on_binop op v1 v2 (Normal v) ->
-    transl_value v1 = OK n1 ->
-    transl_value v2 = OK n2 ->
-    transl_value v = OK n ->
+    transl_value v1 = n1 ->
+    transl_value v2 = n2 ->
+    transl_value v = n ->
     forall m, Cminor.eval_binop (transl_binop op) n1 n2 m = Some n.
 Proof.
   !intros.
   assert (h_rtc:=do_run_time_check_on_binop_ok _ _ _ _ h_do_rtc_binop).
-  destruct op.
-  - erewrite (and_ok v1 v2 v n1 n2) in heq_transl_value;eq_same_clear;eauto.
-  - erewrite (or_ok v1 v2 v n1 n2) in heq_transl_value;eq_same_clear;eauto.
-  - erewrite (eq_ok v1 v2 v n1 n2) in heq_transl_value;eq_same_clear;eauto.
-  - erewrite (neq_ok v1 v2 v n1 n2) in heq_transl_value;eq_same_clear;eauto.
-  - erewrite (lt_ok v1 v2 v n1 n2) in heq_transl_value;eq_same_clear;eauto.
-  - erewrite (le_ok v1 v2 v n1 n2) in heq_transl_value;eq_same_clear;eauto.
-  - erewrite (gt_ok v1 v2 v n1 n2) in heq_transl_value;eq_same_clear;eauto.
-  - erewrite (ge_ok v1 v2 v n1 n2) in heq_transl_value;eq_same_clear;eauto.
-  - erewrite (add_ok v v1 v2 n1 n2) in heq_transl_value;eq_same_clear;eauto.
-  - erewrite (sub_ok v v1 v2 n1 n2) in heq_transl_value;eq_same_clear;eauto.
-  - erewrite (mult_ok v v1 v2 n1 n2) in heq_transl_value;eq_same_clear;eauto.
+  destruct op;simpl.
+  - erewrite (and_ok v1 v2 v n1 n2) in heq_transl_value;eq_same_clear;subst;eauto.
+  - erewrite (or_ok v1 v2 v n1 n2) in heq_transl_value;eq_same_clear;subst;eauto.
+  - erewrite (eq_ok v1 v2 v n1 n2) in heq_transl_value;eq_same_clear;subst;eauto.
+  - erewrite (neq_ok v1 v2 v n1 n2) in heq_transl_value;eq_same_clear;subst;eauto.
+  - erewrite (lt_ok v1 v2 v n1 n2) in heq_transl_value;eq_same_clear;subst;eauto.
+  - erewrite (le_ok v1 v2 v n1 n2) in heq_transl_value;eq_same_clear;subst;eauto.
+  - erewrite (gt_ok v1 v2 v n1 n2) in heq_transl_value;eq_same_clear;subst;eauto.
+  - erewrite (ge_ok v1 v2 v n1 n2) in heq_transl_value;eq_same_clear;subst;eauto.
+  - erewrite (add_ok v v1 v2 n1 n2) in heq_transl_value;eq_same_clear;subst;eauto.
+  - erewrite (sub_ok v v1 v2 n1 n2) in heq_transl_value;eq_same_clear;subst;eauto.
+  - erewrite (mult_ok v v1 v2 n1 n2) in heq_transl_value;eq_same_clear;subst;eauto.
   - simpl in *. erewrite (div_ok v v1 v2 n n1 n2);eauto.
 Qed.
 
@@ -810,47 +873,15 @@ Proof.
 Qed.
   
 
-(* TRYING A NEW VERSION *)
 
-
-Inductive follow_chaining: Values.val -> Memory.Mem.mem -> nat -> Values.val -> Prop :=
-  FC1: forall sp m, follow_chaining sp m 0 sp
-| FC2: forall vsp m lvl vsp' v,
-        Memory.Mem.loadv AST.Mint32 m vsp = Some vsp'
-        -> follow_chaining vsp' m lvl v
-        -> follow_chaining vsp m (S lvl) v.
-
-(** [eq_frame sto b ofs m] means that the memory m contains a block
-    at address b, and this block from offset [ofs] matches the spark
-    frame [sto]. *)
-(* FIXME: are we looking at the stack in the wrong direction? *)
-Inductive eq_frame:
-  STACK.store -> Values.block -> Integers.Int.int -> Memory.Mem.mem -> Prop :=
-  MF1: forall spb ofs m, eq_frame nil spb ofs m
-| MF2: forall fr spb ofs m id vid vid',
-         transl_value vid = OK vid'
-         -> Memory.Mem.load AST.Mint32 m spb ofs = Some vid'
-         -> eq_frame fr spb (Integers.Int.add (Integers.Int.repr ofs)
-                                               (Integers.Int.repr 4)) m
-         -> eq_frame ((id,vid)::fr) spb (Integers.Int.repr ofs) m.
-
-(** [match_env sta b m] means that the chained Cminor stack at address
-    [b] in memory m ([b] is the adress of the bottom of the top stack)
-    matches spark stack [s]. *)
-Inductive eq_env: STACK.stack -> Values.block -> Memory.Mem.mem -> Prop :=
-  ME1: forall spb m, eq_env nil spb m
-| ME2: forall s sto (lvl:STACK.scope_level) fr spb spb' m,
-         eq_frame fr spb (Integers.Int.repr 4) m
-         -> eq_env s spb' m
-         -> eq_env ((lvl,sto)::s) spb m.
-
-
-
-
-
-
-
-
+Definition stack_match st s CE sp locenv g m :=
+  forall nme v addrof_nme load_addrof_nme typ_nme cm_typ_nme,
+    eval_name st s nme (Normal v) ->
+    type_of_name st nme = OK typ_nme ->
+    transl_name st CE nme = OK addrof_nme ->
+    transl_type st typ_nme = OK cm_typ_nme ->
+    make_load addrof_nme cm_typ_nme = OK load_addrof_nme ->
+    Cminor.eval_expr g sp locenv m load_addrof_nme (transl_value v).
 
 (* See CminorgenProof.v@205. *)
 (* We will need more than that probably. But for now let us use
@@ -864,73 +895,24 @@ Inductive eq_env: STACK.stack -> Values.block -> Memory.Mem.mem -> Prop :=
 
    We also put well-typing constraints on the stack wrt symbol
    table. *)
-Record match_env (*st:symboltable*) (s: semantics.STACK.stack)
-       (*CE:compilenv*) (spb:Values.block) (ofs:Integers.Int.int)
-       (*locenv: Cminor.env*) (*g:genv*)(m:Memory.Mem.mem): Prop :=
+
+Record match_env (st:symboltable) (s: semantics.STACK.stack)
+       (CE:compilenv) (sp:Values.val) (locenv: Cminor.env)
+       (g:genv)(m:Memory.Mem.mem): Prop :=
   mk_match_env {
-      me_eq_stack: eq_env s spb m;
-(*       me_eq_locenv: local variable never change in our semantic anyway; *)
-      me_overflow: safe_stack s }.
-
-
-
-Axiom
-      me_transl:
-        forall st s CE spb ofs locenv g m,
-        forall nme v addrof_nme load_addrof_nme typ_nme cm_typ_nme v',
-          eval_name st s nme (Normal v) ->
-          type_of_name st nme = OK typ_nme ->
-          transl_name st CE nme = OK addrof_nme ->
-          transl_type st typ_nme = OK cm_typ_nme ->
-          make_load addrof_nme cm_typ_nme = OK load_addrof_nme ->
-          transl_value v = OK v' ->
-          Cminor.eval_expr g (Values.Vptr spb ofs) locenv m load_addrof_nme v'.
-
+      me_transl: stack_match st s CE sp locenv g m;
+      me_overflow: safe_stack s
+    }.
 
 
 (** Hypothesis renaming stuff *)
 Ltac rename_hyp3 h th :=
   match th with
-    | match_env _ _ _ _ => fresh "h_match_env"
+    | match_env _ _ _ _ _ _ _ => fresh "h_match_env"
     | _ => rename_hyp2 h th
   end.
 
 Ltac rename_hyp ::= rename_hyp3.
-
-
-
-Lemma transl_name_ok :
-  forall stbl (s:STACK.stack) (nme:name) (v:value),
-    eval_name stbl s nme (Normal v) ->
-    forall CE locenv g m  (e' e'':Cminor.expr)
-           typeof_nme typeof_nme' spb ofs v',
-      type_of_name stbl nme = OK typeof_nme ->
-      transl_type stbl typeof_nme = OK typeof_nme' ->
-      transl_name stbl CE nme = OK e' ->
-      match_env s spb ofs m ->
-      make_load e' typeof_nme' = OK e'' ->
-      transl_value v = OK v' ->
-      Cminor.eval_expr g (Values.Vptr spb ofs) locenv m e'' v'.
-Proof.
-  intros until v.
-  intro h_eval_name.
-  remember (Normal v) as Nv.
-  revert HeqNv.
-  !induction h_eval_name;simpl;!intros; subst;try discriminate.
-  !invclear heq.
-  !destruct h_match_env.
-  rename x into i.
-  rename v into val_i.
-  specialize (me_transl st s CE spb ofs locenv g m (E_Identifier ast_num i) val_i e' e''
-                        typeof_nme typeof_nme' v').
-  intro h_me_transl.
-  !! (fun _ => assert (eval_name st s (E_Identifier ast_num i) (Normal val_i))) g.
-  { constructor.
-    assumption. }
-  specialize (h_me_transl h_eval_name heq_fetch_var_type heq_transl_variable
-                         heq_transl_type heq_make_load heq_transl_value).
-  repeat split;auto.
-Qed.
 
 Ltac rename_hyp4 h th :=
   match reverse goal with
@@ -938,13 +920,20 @@ Ltac rename_hyp4 h th :=
     | H: id (fetch_var_type ?X _ = OK h) |- _ => (fresh "type_" X)
     | H: (value_at_addr _ _ ?X = OK h) |- _ => fresh "val_at_" X
     | H: id (value_at_addr _ _ ?X = OK h) |- _ => fresh "val_at_" X
-    | H: transl_variable _ _ _ ?X = OK h |- _ => fresh X "'"
-    | H: id (transl_variable _ _ _ ?X = OK h) |- _ => fresh X "'"
-    | H: transl_value ?X = OK h |- _ => fresh X "'"
-    | H: id (transl_value ?X = OK h) |- _ => fresh X "'"
+    | H: transl_variable _ _ _ ?X = OK h |- _ => fresh X "_t"
+    | H: id (transl_variable _ _ _ ?X = OK h) |- _ => fresh X "_t"
+    | H: transl_value ?X = OK h |- _ => fresh X "_t"
+    | H: id (transl_value ?X = OK h) |- _ => fresh X "_t"
     | _ => rename_hyp3 h th
   end.
 Ltac rename_hyp ::= rename_hyp4.
+
+(* Is this true? *)
+(*Axiom CM_eval_bigstep_det: forall g sp locenv m e v v',
+    Cminor.eval_expr g sp locenv m e v ->
+    Cminor.eval_expr g sp locenv m e v' ->
+    v = v'.*)
+
 
 Lemma transl_expr_ok :
   forall stbl CE (e:expression) (e':Cminor.expr),
@@ -952,90 +941,67 @@ Lemma transl_expr_ok :
     forall locenv g m (s:STACK.stack)  (v:value)
          (spb: Values.block) (ofs:Integers.Int.int),
     eval_expr stbl s e (Normal v) ->
-    match_env s spb ofs m ->
-    forall v',
-    transl_value v = OK v' ->
-    Cminor.eval_expr g (Values.Vptr spb ofs) locenv m e' v'.
+    match_env stbl s CE (Values.Vptr spb ofs) locenv g m ->
+    Cminor.eval_expr g (Values.Vptr spb ofs) locenv m e' (transl_value v).
 Proof.
   intros until e.
   !functional induction (transl_expr stbl CE e);try discriminate;simpl; !intros;
   !invclear h_eval_expr;eq_same_clear.
-  - destruct (transl_literal_ok g lit v h_eval_literal (Values.Vptr spb ofs)) as [vv h_and].
-    !destruct h_and;eq_same_clear.
+  - generalize (transl_literal_ok g lit v h_eval_literal (Values.Vptr spb ofs)).
+    !intro.
     constructor.
     assumption.
-  - rename v'0 into v'.
-    unfold value_at_addr in heq.
+  - unfold value_at_addr in heq.
     destruct (transl_type stbl type_id) eqn:heq_transl_type;simpl in *.
-    + eapply transl_name_ok;simpl; eauto.
+    + !destruct h_match_env.
+      eapply me_transl0;eauto.
     + discriminate.
-  - specialize (IHr x heq0 locenv g m s v1 spb ofs).
-    specialize (IHr0 x0 heq locenv g m s v2 spb ofs).
-    destruct (transl_value v1) as [v1' | errormsg] eqn:heq_transl_value_v1.
-    destruct (transl_value v2) as [v2' | errormsg] eqn:heq_transl_value_v2.
-    + apply eval_Ebinop with v1' v2';auto.
-      eapply binary_operator_ok;eauto.
-      * eapply eval_expr_overf2;eauto.
-        eapply h_match_env.(me_overflow s spb ofs m).
-      * eapply eval_expr_overf2;eauto.
-        eapply h_match_env.(me_overflow s spb ofs m).
-    + functional inversion heq_transl_value_v2;subst.
-      * admit. (* Arrays *)
-      * admit. (* Records *)
-      * admit. (* Undefined *)
-    + functional inversion heq_transl_value_v1;subst.
-      * admit. (* Arrays *)
-      * admit. (* Records *)
-      * admit. (* Undefined *)
+  - specialize (IHr x heq0 locenv g m s v1 spb ofs h_eval_expr0 h_match_env).
+    specialize (IHr0 x0 heq locenv g m s v2 spb ofs h_eval_expr h_match_env).
 
+    eapply eval_Ebinop;eauto. 
+    eapply binary_operator_ok;eauto.
+    * eapply eval_expr_overf2;eauto.
+      eapply h_match_env.(me_overflow stbl s CE (Values.Vptr spb ofs) locenv g m).
+    * eapply eval_expr_overf2;eauto.
+      eapply h_match_env.(me_overflow stbl s CE (Values.Vptr spb ofs) locenv g m).
   (* Unary minus *)
   - simpl in heq.
     eq_same_clear.
     rename x into e'.
     rename e0 into e.
-    destruct (transl_value v0) eqn:heq_transl_value_v
-    ; try discriminate;eq_same_clear;simpl in *.
     specialize (IHr e' heq0 locenv g m s v0 spb ofs
-                    h_eval_expr h_match_env v1 heq_transl_value_v).
-    + apply eval_Eunop with (v1:=v1);auto.
-      simpl.
-      assert (h:=unaryneg_ok v1 v0 v heq_transl_value_v).
-      rewrite h in heq_transl_value.
-      * eq_same_clear.
-        reflexivity.
-      * simpl in *.
-        { !invclear h_do_rtc_unop; simpl in *.
-          - !invclear h_overf_check;subst;simpl in *; try eq_same_clear.
-            assumption.
-          - assumption. }
-    + functional inversion heq_transl_value_v;subst.
-      * inversion h_do_rtc_unop;subst; simpl in *;try discriminate.
-      * inversion h_do_rtc_unop;subst; simpl in *;try discriminate.
-      * inversion h_do_rtc_unop;subst; simpl in *;try discriminate.
+                    h_eval_expr h_match_env).
+    eapply eval_Eunop;auto.
+    + apply IHr.
+    + simpl.
+      assert (h:=unaryneg_ok (transl_value v0) v0 v eq_refl).
+      rewrite h in *;auto.
+      !invclear h_do_rtc_unop; simpl in *;auto.
+      !invclear h_overf_check;subst;simpl in *; try eq_same_clear.
+      assumption.
   (* Not *)
   - !invclear h_do_rtc_unop;simpl in *;try eq_same_clear.
     clear hneq.
     destruct v0;simpl in *;try discriminate;eq_same_clear;simpl in *.
     destruct n;simpl in *; eq_same_clear.
-    * { econstructor;simpl in *;eauto.
-        * eapply IHr ;eauto.
+    * { econstructor;simpl in *.
+        * eapply IHr;eauto.
+        * econstructor.
           simpl.
-          eauto.
-        * constructor.
-          simpl.
-          eauto.
+          reflexivity.
         * vm_compute.
           reflexivity. }
-    * { econstructor;simpl in *;eauto.
+    * { econstructor;simpl in *.
         * eapply IHr ;eauto.
-          simpl.
-          eauto.
         * constructor.
           simpl.
           eauto.
         * vm_compute.
           reflexivity. }
 Qed.
+
+
 (** Hypothesis renaming stuff *)
 Ltac rename_hyp5 th :=
   match th with
@@ -1050,20 +1016,686 @@ Ltac rename_hyp ::= rename_hyp5.
 Require Import Utf8.
 Set Printing Width 90.
 
+
+Axiom expression_dec: forall e1 e2:expression, ({e1=e2} + {e1<>e2}).
+Axiom name_dec: forall e1 e2:name, {e1=e2} + {e1<>e2}. 
+
+Import STACK.
+
 Axiom det_eval_expr: forall g spb ofs locenv m e v v',
                        Cminor.eval_expr g (Values.Vptr spb ofs) locenv m e v
                        -> Cminor.eval_expr g (Values.Vptr spb ofs) locenv m e v'
                        -> v = v'.
+
+Inductive le_loads (lds: Cminor.expr): Cminor.expr -> Prop :=
+  le_loads_n: le_loads lds lds
+| le_loads_L: ∀ lds', le_loads lds lds' -> le_loads lds (Eload AST.Mint32 lds').
+ 
+Definition lt_loads := λ l₁ l₂, le_loads(Eload AST.Mint32 l₁) l₂.
+
+Lemma le_loads_ese_L : forall lds₁ lds₂: Cminor.expr,
+    le_loads lds₁ lds₂ -> le_loads (Eload AST.Mint32 lds₁) (Eload AST.Mint32 lds₂).
+Proof.
+  !intros.
+  induction H.
+  - constructor 1.
+  - constructor 2.
+    assumption.
+Qed.
+
+Lemma le_load_L_e : ∀ l₁ l₂,
+    le_loads (Eload AST.Mint32 l₁) (Eload AST.Mint32 l₂) ->
+    le_loads l₁ l₂.
+Proof.
+  intros l₁ l₂.
+  revert l₁.
+  induction l₂;intros;try discriminate.
+  - inversion H;try now constructor.
+    inversion H1.
+  - inversion H;try now constructor.
+    inversion H1.
+  - inversion H;try now constructor.
+    inversion H1.
+  - inversion H;try now constructor.
+    inversion H1.
+  - inversion H;try now constructor.
+    inversion H1;subst.
+    + constructor 2.
+      auto.
+    + constructor 2.
+      auto.
+Qed.
+
+Lemma lt_load_L_L : ∀ l₁ l₂,
+    lt_loads (Eload AST.Mint32 l₁) (Eload AST.Mint32 l₂) ->
+    lt_loads l₁ l₂.
+Proof.
+  unfold lt_loads.
+  intros l₁ l₂ H.
+  apply le_load_L_e;auto.
+Qed.
+
+Lemma lt_load_irrefl : ∀ l₁, ¬ lt_loads l₁ l₁.
+Proof.
+  intros l₁.
+  unfold lt_loads.
+  induction l₁;try (intro abs; inversion abs).
+  - subst m.
+    apply IHl₁.
+    rewrite <- H1 at 2.
+    constructor 1.
+  - subst.
+    apply le_load_L_e in abs.
+    apply IHl₁.
+    assumption.
+Qed.
+
+Lemma lt_load_neq : ∀ l₁ l₂, lt_loads l₁ l₂ -> l₁ ≠ l₂.
+Proof.
+  unfold lt_loads.
+  intros l₁ l₂.
+  remember (Eload AST.Mint32 l₁) as h'.
+  revert h' l₁ Heqh'.
+  induction l₂;intros; subst ; try now inversion H.
+  intro abs.
+  subst.
+  assert (m=AST.Mint32). {
+    inversion H;auto. }
+  subst.
+  apply le_load_L_e in H.
+  specialize (IHl₂ (Eload AST.Mint32 l₂) l₂ eq_refl H).
+  apply IHl₂;auto.
+Qed.
+
+
+Lemma neq_sym : forall A, forall x y : A , x<>y  -> y<>x.
+Proof.
+  intros A x y H.
+  intro abs.
+  subst.
+  apply H;reflexivity.
+Qed.
+
+Lemma build_loads__inj :
+  forall i₁ i₂,
+    (* translating the variabe to a Cminor load address *)
+    build_loads_ i₁ = build_loads_ i₂ ->
+    i₁ = i₂.
+Proof.
+  intros i₁.
+  !induction i₁;simpl;!intros.
+  - destruct i₂;auto.
+    simpl in heq.
+    inversion heq.
+  - destruct  i₂;simpl in *;auto.
+    + inversion heq.
+    + inversion heq.
+      rewrite (IHi₁ i₂);auto.
+Qed.
+
+Lemma build_loads__inj_lt :
+  forall i₁ i₂,
+    (i₁ < i₂)%nat ->
+    forall e₁ e₂ ,
+      (* translating the variabe to a Cminor load address *)
+      build_loads_ i₁ = e₁ ->
+      (* translating the variabe to a Cminor load address *)
+      build_loads_ i₂ = e₂ ->
+      lt_loads e₁ e₂.
+Proof.
+  intros i₁ i₂.
+  unfold lt_loads.
+  !intro.
+  induction H;simpl;!intros;subst.
+  - constructor 1.
+  - constructor 2.
+    apply IHle;auto.
+Qed.
+
+Lemma build_loads__inj_neq :
+  forall i₁ i₂,
+    i₁ ≠ i₂ ->
+    forall e₁ e₂ ,
+      (* translating the variabe to a Cminor load address *)
+      build_loads_ i₁ = e₁ ->
+      (* translating the variabe to a Cminor load address *)
+      build_loads_ i₂ = e₂ ->
+      e₁ ≠ e₂.
+Proof.
+  !intros.
+  intro abs.
+  subst.
+  apply build_loads__inj in abs.
+  contradiction.
+Qed.
+
+Lemma build_loads_inj :
+  forall i₁ i₂ k k' ,
+      (* translating the variabe to a Cminor load address *)
+      build_loads k i₁ = build_loads k' i₂ ->
+      k = k' ∧ Integers.Int.Z_mod_modulus i₁ = Integers.Int.Z_mod_modulus i₂.
+Proof.
+  unfold build_loads.
+  !intros.
+  inversion heq.
+  split;auto.  
+  apply build_loads__inj;auto.
+Qed.
+
+Lemma build_loads_inj_neq1 :
+  forall i₁ i₂ k k' e₁ e₂,
+    k ≠ k' ->
+    build_loads k i₁ = e₁ ->
+    build_loads k' i₂ = e₂ ->
+    e₁ ≠ e₂.
+Proof.
+  !intros.
+  intro abs.
+  subst.
+  apply build_loads_inj in abs.
+  destruct abs;contradiction.
+Qed.
+
+Lemma build_loads_inj_neq2 :
+  forall i₁ i₂ k k' e₁ e₂,
+    Integers.Int.Z_mod_modulus i₁ ≠ Integers.Int.Z_mod_modulus i₂ ->
+    build_loads k i₁ = e₁ ->
+    build_loads k' i₂ = e₂ ->
+    e₁ ≠ e₂.
+Proof.
+  !intros.
+  intro abs.
+  subst.
+  apply build_loads_inj in abs.
+  destruct abs;contradiction.
+Qed.
+
+
+Lemma CEfetch_reside_true : forall id a x,
+    CompilEnv.fetch id a = Some x -> CompilEnv.reside id a = true.
+Proof.
+  intros until a.
+  unfold CompilEnv.fetch, CompilEnv.reside.
+  induction (CompilEnv.store_of a);simpl;!intros;try discriminate.
+  destruct a0.
+  destruct (beq_nat id i).
+  - reflexivity.
+  - eapply IHs;eauto.
+Qed.
+
+Lemma CEfetch_reside_false : forall id a,
+    CompilEnv.fetch id a = None -> CompilEnv.reside id a = false.
+Proof.
+  intros until a.
+  unfold CompilEnv.fetch, CompilEnv.reside.
+  induction (CompilEnv.store_of a);simpl;!intros;try reflexivity.
+  destruct a0.
+  destruct (beq_nat id i).
+  - discriminate.
+  - eapply IHs;eauto.
+Qed.
+
+
+
+Lemma frameG_In : forall a id st,
+    CompilEnv.frameG id a = Some st ->
+    List.In st a.
+Proof.
+  intro a.
+  !induction a;simpl;intros;try discriminate.
+  !destruct (CompilEnv.reside id a).
+  - inversion H.
+    left.
+    reflexivity.
+  - right.
+    eapply IHa;eauto.
+Qed.
+
+Lemma fetches_In : forall a id st,
+    CompilEnv.fetches id a = Some st ->
+    List.In (id,st) a.
+Proof.
+  intro a.
+  !induction a;simpl;!intros;try discriminate.
+  !destruct a;simpl in *.
+  !destruct (eq_nat_dec id i);subst;simpl in *.
+  - rewrite <- beq_nat_refl in heq.
+    inversion heq.
+    left.
+    reflexivity.
+  - right.
+    rewrite <- beq_nat_false_iff in hneq.
+    rewrite hneq in heq.
+    eapply IHa;eauto.
+Qed.
+
+Lemma fetch_In : forall a id st,
+    CompilEnv.fetch id a = Some st ->
+    List.In (id,st) (CompilEnv.store_of a).
+Proof.
+  !intros.
+  unfold CompilEnv.fetch in heq_CEfetch_id_a.
+  apply fetches_In.
+  assumption.
+Qed.
+
+
+
+
+Require Import FMapList.
+Require Import OrderedType.
+
+(*
+Inductive increasing_order : localframe -> Prop :=
+  IncO : increasing_order []
+| IncNext: forall lf id δ,
+    increasing_order lf ->
+    (forall otherid y', CompilEnv.fetches otherid lf = Some y' -> δ < y') ->
+    increasing_order ((id,δ)::lf).
+*)
+(*
+Module localframeORD <: OrderedType.
+  Definition t := (idnum * CompilEnv.V)%type.
+  
+  Definition eq := @eq t.
+  Definition lt := (fun x y:t => snd x < snd y).
+
+  Definition eq_refl := @eq_refl t.
+  Definition eq_sym := @eq_sym t.
+  Definition eq_trans := @eq_trans t.
+  Opaque eq_refl eq_sym eq_trans.
+
+  Lemma lt_not_eq : forall m1 m2 : t, lt m1 m2 -> ~ eq m1 m2.
+  Proof.
+    !intros.
+    unfold eq , lt in *.
+    intro abs.
+    subst.
+    destruct (Z.lt_irrefl _ H).
+  Qed.
+  Lemma lt_irrefl: bool.
+    exact true.
+  Qed.
+  Lemma lt_antisym :symmetric _ lt.
+  Proof.
+    admit.
+  Qed.
+      
+  Lemma lt_trans:transitive _ lt.
+  Proof.
+    unfold transitive.
+    !intros.
+    unfold lt in *.
+    eapply Zlt_trans;eauto.
+  Qed.
+
+
+
+End localframeORD.
+MSetList.Make().
+*)
+Definition increasing_order: localframe -> Prop := StronglySorted (fun x y => snd x > snd y).
+
+Definition increasing_order_fr (f:CompilEnv.frame) :=
+  increasing_order(CompilEnv.store_of f).
+
+
+(* FIXME: find another name *)
+(* levels of each substack are ordered *)
+(*
+Inductive increasing_orderG : CompilEnv.stack -> Prop :=
+  IncOG : increasing_orderG []
+| IncNextG: forall stk frm,
+    increasing_orderG stk ->
+    increasing_order_fr frm ->
+    (List.Forall
+       (fun otherfrm =>
+          (CompilEnv.level_of otherfrm < CompilEnv.level_of frm)%nat)
+       stk) ->
+    increasing_orderG (frm::stk).
+*)
+Definition increasing_orderG (stk: CompilEnv.stack): Prop :=
+  StronglySorted (fun x y => (CompilEnv.level_of x > CompilEnv.level_of y)%nat) stk.
+
+
+
+
+Ltac rename_hyp_incro h th :=
+  match th with
+    | increasing_order_fr ?x => fresh "h_incr_order_fr_" x
+    | increasing_order_fr _ => fresh "h_incr_order_fr"
+    | increasing_order ?x => fresh "h_incr_order_" x
+    | increasing_order _ => fresh "h_incr_order"
+    | increasing_orderG ?x => fresh "h_incr_orderG_" x
+    | increasing_orderG _ => fresh "h_incr_orderG"
+    | Forall ?P ?x => fresh "h_forall_" P "_" x
+    | Forall _ ?x => fresh "h_forall_" x
+    | Forall ?P _ => fresh "h_forall_" P
+    | Forall _ _ => fresh "h_forall"
+    | _ => rename_hyp5 h th
+  end.
+Ltac rename_hyp ::= rename_hyp_incro.
+
+Section mapping.
+  
+  Variable (stbl: symboltable) (CE:compilenv) (ofs : Integers.Int.int)
+           (spb : Values.block) (locenv : env) (g : genv).
+
+  Lemma increase_order_level_of_top_ge:
+    forall id s s0 s3,
+      increasing_orderG CE ->
+      CompilEnv.frameG id CE = Some (s, s0) ->
+      CompilEnv.level_of_top CE = Some s3 -> 
+      (s3 >= s)%nat.
+  Proof.
+    !intros.
+    unfold increasing_orderG in *.
+    !destruct CE;!intros.
+    - simpl in *;try discriminate.
+    - specialize (increasing_order_In _ _ _ _ h_incr_orderG_CE).
+      !intro.
+      rewrite Forall_forall in h_forall.
+      apply NPeano.Nat.lt_eq_cases.
+      unfold CompilEnv.level_of in *.
+      apply frameG_In in heq_CEframeG_id_CE.
+      specialize (h_forall _ heq_CEframeG_id_CE).
+      !destruct f.
+      unfold CompilEnv.level_of_top in heq_lvloftop_CE_s3.
+      simpl in *.
+      !invclear heq_lvloftop_CE_s3.
+      !destruct h_forall;auto.
+      inject heq;auto.
+  Qed.        
+
+  
+  Lemma CEfetches_inj : forall id₁ id₂ (lf:localframe) δ₁ δ₂,
+      increasing_order lf ->
+      CompilEnv.fetches id₁ lf = Some δ₁ ->
+      CompilEnv.fetches id₂ lf = Some δ₂ ->
+      id₁ ≠ id₂ ->
+      δ₁ ≠ δ₂.
+  Proof.
+    intros until lf.
+    !induction lf;simpl in *;!intros.
+    - discriminate.
+    - destruct a.
+      destruct (NPeano.Nat.eq_dec id₁ i);subst.
+      + rewrite NPeano.Nat.eqb_refl in heq0.
+        !invclear heq0.
+        assert (h:id₂ ≠ i) by auto.
+        rewrite <- (NPeano.Nat.eqb_neq id₂ i) in h.
+        rewrite h in heq.
+        inversion h_incr_order;subst;simpl in *.
+        assert (δ₁ > δ₂). {
+          rewrite Forall_forall in H2.
+          eapply (H2 (id₂,δ₂));eauto.
+          apply fetches_In.
+          assumption. }
+        apply neq_sym.
+        apply Z.lt_neq.
+        apply Z.gt_lt_iff.
+        assumption.
+      + destruct (NPeano.Nat.eq_dec id₂ i).
+        * subst.        
+          rewrite NPeano.Nat.eqb_refl in heq.
+          !invclear heq.
+          assert (h:id₁ ≠ i) by auto.
+          rewrite <- (NPeano.Nat.eqb_neq id₁ i) in h.
+          rewrite h in heq0.
+          inversion h_incr_order;subst;simpl in *.
+        assert (δ₂ > δ₁). {
+          rewrite Forall_forall in H2.
+          eapply (H2 (id₁,δ₁));eauto.
+          apply fetches_In.
+          assumption. }
+        apply Z.lt_neq.
+        apply Z.gt_lt_iff.
+        assumption.
+        * rewrite <- (NPeano.Nat.eqb_neq id₁ i) in n.
+          rewrite <- (NPeano.Nat.eqb_neq id₂ i) in n0.
+          rewrite n,n0 in *.
+          apply IHlf;auto.
+          inversion h_incr_order.
+          assumption.
+  Qed.
+
+  
+  Lemma CEfetch_inj : forall id₁ id₂ (a:CompilEnv.frame) δ₁ δ₂,
+      increasing_order_fr a -> 
+      CompilEnv.fetch id₁ a = Some δ₁ ->
+      CompilEnv.fetch id₂ a = Some δ₂ ->
+      id₁ ≠ id₂ ->
+      δ₁ ≠ δ₂.
+  Proof.
+    intros until a.
+    unfold CompilEnv.fetch.
+    !destruct a;simpl.
+    unfold increasing_order_fr.
+    simpl.
+    apply CEfetches_inj.
+  Qed.
+
+
+  Lemma CEfetchG_inj : forall id₁ id₂,
+      increasing_orderG CE -> 
+      List.Forall (fun otherfrm => increasing_order_fr otherfrm) CE ->
+      forall  δ₁ δ₂ k₁ k₂ frm₁ frm₂,
+        CompilEnv.fetchG id₁ CE = Some δ₁ ->
+        CompilEnv.fetchG id₂ CE = Some δ₂ ->
+        CompilEnv.frameG id₁ CE = Some (k₁, frm₁) -> 
+        CompilEnv.frameG id₂ CE = Some (k₂, frm₂) -> 
+        id₁ ≠ id₂ ->
+        (k₁ <> k₂ \/ δ₁ <> δ₂).
+  Proof.
+    intros id₁ id₂.
+    !intro.
+    !induction h_incr_orderG_CE;!intros;simpl in *;try discriminate.
+    rewrite Forall_forall in h_forall_l, h_forall.
+    unfold CompilEnv.level_of in *.
+    destruct (CompilEnv.fetch id₁ a) eqn:heq_fetch_id₁;
+      destruct (CompilEnv.fetch id₂ a) eqn:heq_fetch_id₂;
+      eq_same_clear;subst;simpl in *;try discriminate.
+    - right.
+      eapply CEfetch_inj;eauto.
+    - left.
+      apply neq_sym.
+      apply NPeano.Nat.lt_neq.
+      apply CEfetch_reside_false in heq_fetch_id₂.
+      apply CEfetch_reside_true in heq_fetch_id₁.
+      rewrite heq_fetch_id₂,heq_fetch_id₁ in *;simpl in *.
+      !invclear heq_CEframeG_id₁;simpl in *.
+      specialize (h_forall_l (k₂, frm₂)).
+      simpl in *.
+      apply h_forall_l.
+      eapply frameG_In;eauto.
+    - left.
+      apply NPeano.Nat.lt_neq.
+      apply CEfetch_reside_true in heq_fetch_id₂.
+      apply CEfetch_reside_false in heq_fetch_id₁.
+      rewrite heq_fetch_id₂,heq_fetch_id₁ in *;simpl in *.
+      !invclear heq_CEframeG_id₂;simpl in *.
+      specialize (h_forall_l (k₁, frm₁)).
+      simpl in *.
+      apply h_forall_l.
+      eapply frameG_In;eauto.
+    - apply CEfetch_reside_false in heq_fetch_id₁. 
+      apply CEfetch_reside_false in heq_fetch_id₂. 
+      rewrite heq_fetch_id₁,heq_fetch_id₂ in *.
+      eapply IHh_incr_orderG_CE ;eauto.
+      rewrite Forall_forall.
+      intros x H.
+      apply h_forall;auto.
+  Qed.
+
+
+  Lemma minus_same_eq : forall s3 s s1,
+    s ≤ s3 ->
+    s1 ≤ s3 ->
+    (s3 - s1)%nat = (s3 - s)%nat ->
+    s = s1.
+  Proof.
+    induction s3;intros.
+    - inversion H0;inversion H;auto.
+    - inversion H;inversion H0;subst.
+      + reflexivity.
+      + rewrite minus_diag in H1.
+        apply NPeano.Nat.sub_0_le in H1.
+        assert (s3 < s3)%nat. {
+          eapply lt_le_trans with s1;auto. }
+        destruct (lt_irrefl s3);auto.
+      + rewrite minus_diag in H1.
+        symmetry in H1.
+        apply NPeano.Nat.sub_0_le in H1.
+        assert (s3 < s3)%nat. {
+          eapply lt_le_trans with s;auto. }
+        destruct (lt_irrefl s3);auto.
+      + eapply IHs3;eauto.
+        setoid_rewrite <- minus_Sn_m in H1;auto.
+  Qed.
+
+  Lemma minus_same_neq : forall s3 s s1,
+    s ≤ s3 ->
+    s1 ≤ s3 ->
+    s <> s1 ->
+    (s3 - s1)%nat <> (s3 - s)%nat.
+  Proof.
+    !intros.
+    intro abs.
+    apply minus_same_eq in abs;auto.
+  Qed.
+
+
+  
+  Lemma foo :
+    forall a₁ a₂ id₁ id₂ k₁ k₂ δ₁ δ₂,
+      (* Frame are numbered with different (increasing) numers *)
+      increasing_orderG CE ->
+      (* In each frame, stacks are also numbered with (increasing) numbers *)
+      List.Forall (fun otherfrm => increasing_order_fr otherfrm) CE ->
+      (forall id δ, CompilEnv.fetchG id CE = Some δ -> 0 <= δ ∧ δ < Integers.Int.modulus) ->
+      (* translating the variabe to a Cminor load address *)
+      transl_variable stbl CE a₁ id₁ = OK (build_loads k₁ δ₁) ->
+      (* translating the variabe to a Cminor load address *)
+      transl_variable stbl CE a₂ id₂ = OK   (build_loads k₂ δ₂) ->
+      id₁ <> id₂ ->
+      (k₁ <> k₂ \/ δ₁<> δ₂).
+  Proof.
+    !intros.
+    match goal with
+    | H: appcontext [(0 <= _) ∧ (_ < Integers.Int.modulus)] |- _ => rename H into h_bound_CE
+    end.
+    unfold transl_variable in *.
+    destruct (CompilEnv.fetchG id₁ CE) eqn:h₁;simpl in *;try discriminate.
+    destruct (CompilEnv.fetchG id₂ CE) eqn:h₂;simpl in *;try discriminate.
+    destruct (CompilEnv.frameG id₁ CE) eqn:h₁';simpl in *;try discriminate.
+    destruct (CompilEnv.frameG id₂ CE) eqn:h₂';simpl in *;try discriminate.
+    destruct f.
+    destruct f0.
+    assert (hh:=CEfetchG_inj _ _ h_incr_orderG_CE h_forall_CE _ _ _ _ _ _  h₁ h₂ h₁' h₂' hneq).
+    destruct (CompilEnv.level_of_top CE) eqn:hlvlofCE.
+    - (* remember here refrain inversion to bizarrely unfold too much. *)
+      remember (build_loads (s3 - s1) t0) as fooo.
+      remember (build_loads (s3 - s) t) as fooo'.
+      inversion heq_transl_variable as [heqfoo].
+      inversion heq_transl_variable0 as [heqfoo'].
+      clear heq_transl_variable heq_transl_variable0.
+      subst.
+      apply build_loads_inj in heqfoo.
+      apply build_loads_inj in heqfoo'.
+      !destruct heqfoo.
+      !destruct heqfoo'.
+      subst.
+      !destruct hh.
+      + left.
+        eapply minus_same_neq;eauto.
+        eapply increase_order_level_of_top_ge;eauto.
+        eapply increase_order_level_of_top_ge;eauto.
+      + repeat rewrite Integers.Int.Z_mod_modulus_eq in *.
+        rewrite Coqlib.Zmod_small in *;eauto.
+        subst.
+        right.
+        intro abs.
+        subst.
+        apply hneq0;reflexivity.
+    - discriminate.
+  Qed.
+
+
+  (* We need something more precise, probably this: *)
+  Lemma foo2 :
+    forall stbl chnk₁ chnk₂ a₁ a₂ id₁ id₂ k₁ k₂ δ₁ δ₂,
+      (* Frame are numbered with different (increasing) numers *)
+      increasing_orderG CE ->
+      (* In each frame, stacks are also numbered with (increasing) numbers *)
+      List.Forall (fun otherfrm => increasing_order_fr otherfrm) CE ->
+      (forall id δ, CompilEnv.fetchG id CE = Some δ
+                    -> 0 <= δ ∧ δ < Integers.Int.modulus) ->
+      (* translating the variabe to a Cminor load address *)
+      transl_variable stbl CE a₁ id₁ = OK (build_loads k₁ δ₁) ->
+      (* translating the variabe to a Cminor load address *)
+      transl_variable stbl CE a₂ id₂ = OK (build_loads k₂ δ₂) ->
+      compute_chnk_id stbl id₁ = OK chnk₁ ->
+      compute_chnk_id stbl id₂ = OK chnk₂ ->
+      id₁ <> id₂ ->
+      (k₁ <> k₂
+       \/ δ₁ < δ₂ + Memdata.size_chunk chnk₂
+       \/ δ₂ < δ₁ + Memdata.size_chunk chnk₁).
+  Proof.
+  Admitted.
+
+  xxx
+  
+(* storeUpdate stbl s (E_Identifier a i) e0_v (@Normal stack s') *)
+Lemma foo :
+  forall s m a x1 id id_t e e_t e_v e_t_v idaddr s' m',
+    (* translating the variabe to a Cminor load address *)
+    transl_variable stbl CE a id = OK id_t ->
+    (* translating the expression to Cminor *)
+    transl_expr stbl CE e = OK e_t ->
+    (* Evaluating in spark *)
+    eval_expr stbl s e (Normal e_v) ->
+    (* Evaluating expression in Cminor *)
+    Cminor.eval_expr g (Values.Vptr spb ofs) locenv m e_t e_t_v ->
+    (* Evaluating var address in Cminor *)
+    Cminor.eval_expr g (Values.Vptr spb ofs) locenv m id_t idaddr ->
+    (* Size of variable in Cminor memorry *)
+    compute_chnk stbl (E_Identifier a id) = OK x1 ->
+
+    (* the two storing operation maintain match_env *)
+    storeUpdate stbl s (E_Identifier a id) e_v (Normal s') ->
+    Memory.Mem.storev x1 m idaddr e_t_v = Some m' ->
+    match_env stbl s CE (Values.Vptr spb ofs) locenv g m ->
+    match_env stbl s' CE (Values.Vptr spb ofs) locenv g m'.
+
+Proof.
+  intros s m a x1 id id_t e e_t e_v e_t_v idaddr s' m'.
+  !intros.
+  generalize (transl_expr_ok _ _ _ _ heq1).
+  intro h.
+  specialize (h _ _ _ _ _ _ _ h_eval_expr h_match_env).
+
+  unfold transl_variable in heq_transl_variable.
+  destruct (CompilEnv.fetchG id CE) eqn:heqG;try discriminate.
+  destruct (CompilEnv.frameG id CE) eqn:heqfG;try discriminate.
+  destruct f.
+  destruct (CompilEnv.level_of_top CE) eqn:heqlT;simpl in *;try discriminate.
+  
+  
+  admit.
+Qed.
+
+
+
 Lemma transl_stmt_ok :
   forall stbl CE  (stm:statement) (stm':Cminor.stmt),
     transl_stmt stbl CE stm = (OK stm') ->
-    forall locenv g m (s:STACK.stack)
-           (s':STACK.stack) spb ofs f,
-      match_env s spb ofs m ->
+    forall locenv (g:genv) (m:Memory.Mem.mem) (s:stack)
+           (s':stack) (spb:Values.block) ofs f,
+      match_env stbl s CE (Values.Vptr spb ofs) locenv g m ->
       eval_stmt stbl s stm (Normal s') ->
       forall tr locenv' m' o,
         Cminor.exec_stmt g f (Values.Vptr spb ofs) locenv m stm' tr locenv' m' o
-        ->  match_env s' spb ofs m'.
+        ->  match_env stbl s' CE (Values.Vptr spb ofs) locenv g m'.
 Proof.
   intros until stm.
   !functional induction (transl_stmt stbl CE stm)
@@ -1073,7 +1705,90 @@ Proof.
     !invclear h_exec_stmt.
     assumption.
     (* assignment *)
-  - !invclear h_eval_stmt.
+  - rename x into e0_t.
+    rename x0 into nme_t.
+    remember (Values.Vptr spb ofs) as stkpter.
+    !invclear h_eval_stmt.
+    + rename v into e0_v.
+      !invclear h_exec_stmt.
+      rename v into e0_t_v.
+      destruct nme.
+      subst.
+
+      assert (forall CE stkpter locenv' g stbl s a i e0_v s' x1 m vaddr e0_t_v  m'  ,
+                 storeUpdate stbl s (E_Identifier a i) e0_v (Normal s') ->
+                 transl_expr stbl CE e0 = OK e0_t ->
+                 eval_expr stbl s e0 (Normal e0_v) ->
+                 Cminor.eval_expr g stkpter locenv' m e0_t e0_t_v ->
+                 Cminor.eval_expr g stkpter locenv' m nme_t vaddr ->
+                 Memory.Mem.storev x1 m vaddr e0_t_v = Some m' ->
+                 match_env stbl s CE stkpter locenv' g m ->
+                 match_env stbl s' CE stkpter locenv' g m').
+      { admit. }
+      eapply H;eauto.
+      
+
+      
+      * rename i into idnme.
+        generalize (storeUpdate_id_ok_others a stbl s idnme e0_v s' h_storeupdate).
+        intro h_fetch_other_OK.
+        generalize (storeUpdate_id_ok_same a stbl s idnme e0_v s' h_storeupdate).
+        intro h_fetch_same_OK.
+        split. {
+          - red.
+            !intros.
+            rename nme into newnme.
+            destruct (name_dec (E_Identifier a idnme) newnme).
+            + admit. (* address is the same *)
+            + 
+        }
+          
+          * !destruct h_match_env.
+        
+      
+      assert (h:exists v', transl_value e0_v = OK v'). {
+        admit. (* transl_value should not return Error. *)
+      }
+      !destruct h.
+      assert ().
+      
+      eapply transl_expr_ok in heq_transl_value.
+      * 
+      assert (exists v', transl_value e0_v = OK v'). {      
+        transl_expr_ok
+        erewrite CM_eval_bigstep_det in h_CM_eval_expr.
+        - assumption.
+        
+      }.
+      
+      assert (transl_value e0_v = OK v). {
+        transl_expr_ok
+        erewrite CM_eval_bigstep_det in h_CM_eval_expr.
+        - assumption.
+        
+      }
+        
+ 
+          
+          
+        
+        specialize (transl_name_ok stbl s x2 arrObj h_eval_name CE locenv' g m).
+      * specialize (transl_name_ok stbl s x2 arrObj h_eval_name CE locenv' g m).
+        !inversion heq_transl_name.
+        intros h.
+Lemma storeUpdate_ok_same:
+  forall stbl CE s nme nme_t x (v:value) v' s',
+    eval_name stbl s nme (Normal x) ->
+    transl_name stbl CE nme = nme_t ->
+    storeUpdate stbl s nme v (Normal s') ->
+    fetchG nme s' = v ->
+    transl_value v v_t ->
+    Memory.Mem.storev m nme_t v_t m' ->
+    Memory.Mem.loadv chunk m nme_t = Some v_t.
+Proof.
+    
+
+
     specialize (storeUpdate_ok_others ).
 
 
@@ -1154,3 +1869,4 @@ admit.
       want ultimately. *)
 Qed.
 
+*)
